Worked with Cezar to add open and close file to STLC. Starting thinking about how to recast traces in different histories.

rupicola/io/BaseTypes.fst
@@ -1,3 +1,4 @@
 module BaseTypes
 
 type resexn a = either a unit
+type file_descr = nat
